grammatik/Grammatik.lean
@@ -244,6 +244,8 @@ import Grammatik.Zielsatz.SpecProben
 import Grammatik.Zielsatz.RuheNutzer
 import Grammatik.Zielsatz.Beweis
 import Grammatik.Zielsatz.Proben
+import Grammatik.EinpassenVoll
+import Grammatik.Zielsatz.ProbenG1
 import Grammatik.Parser.UebersetzeAllg2
 import Grammatik.ZielOrtInvGrund
 import Grammatik.Fortschritt
