grammatik/Grammatik/HoareRegeln.lean
@@ -694,7 +694,7 @@ theorem stmtOhneRuf_Runabhaengig {l : Bool} {Γ : Ctx} {Λ Λ' : List (Res D)}
     (fun r hk rest hr ihr σ ρ => by
         have hr' : ∀ (σ : World D) (ρ : Env D _), _ := fun σ ρ => ihr σ ρ
         simp only [execBlock]
-        cases hein : einpassen (D.rtyp r) (O.regLies r σ) with
+        cases hein : einpassen O.zeiger (D.rtyp r) (O.regLies r σ) with
         | none => simp only [hein]
         | some v =>
             simp only [hein]
@@ -706,7 +706,7 @@ theorem stmtOhneRuf_Runabhaengig {l : Bool} {Γ : Ctx} {Λ Λ' : List (Res D)}
         have hr' : ∀ (σ : World D) (ρ : Env D _), _ := fun σ ρ => ihr σ ρ
         have he' : ∀ (σ : World D) (ρ : Env D _), _ := fun σ ρ => ihe σ ρ
         simp only [execBlock]
-        cases hein : einpassen (D.rtyp r) (O.regLies r σ) with
+        cases hein : einpassen O.zeiger (D.rtyp r) (O.regLies r σ) with
         | none => simp only [hein]
         | some v =>
             simp only [hein]
@@ -918,7 +918,7 @@ theorem blockOhneRuf_Runabhaengig {l : Bool} {Γ : Ctx} {Λ Λ' : List (Res D)}
     (fun r hk rest hr ihr σ ρ => by
         have hr' : ∀ (σ : World D) (ρ : Env D _), _ := fun σ ρ => ihr σ ρ
         simp only [execBlock]
-        cases hein : einpassen (D.rtyp r) (O.regLies r σ) with
+        cases hein : einpassen O.zeiger (D.rtyp r) (O.regLies r σ) with
         | none => simp only [hein]
         | some v =>
             simp only [hein]
@@ -930,7 +930,7 @@ theorem blockOhneRuf_Runabhaengig {l : Bool} {Γ : Ctx} {Λ Λ' : List (Res D)}
         have hr' : ∀ (σ : World D) (ρ : Env D _), _ := fun σ ρ => ihr σ ρ
         have he' : ∀ (σ : World D) (ρ : Env D _), _ := fun σ ρ => ihe σ ρ
         simp only [execBlock]
-        cases hein : einpassen (D.rtyp r) (O.regLies r σ) with
+        cases hein : einpassen O.zeiger (D.rtyp r) (O.regLies r σ) with
         | none => simp only [hein]
         | some v =>
             simp only [hein]
@@ -1142,7 +1142,7 @@ theorem endOhneRuf_Runabhaengig {l : Bool} {Γ : Ctx} {Λ : List (Res D)}
     (fun r hk rest hr ihr σ ρ => by
         have hr' : ∀ (σ : World D) (ρ : Env D _), _ := fun σ ρ => ihr σ ρ
         simp only [execBlock]
-        cases hein : einpassen (D.rtyp r) (O.regLies r σ) with
+        cases hein : einpassen O.zeiger (D.rtyp r) (O.regLies r σ) with
         | none => simp only [hein]
         | some v =>
             simp only [hein]
@@ -1154,7 +1154,7 @@ theorem endOhneRuf_Runabhaengig {l : Bool} {Γ : Ctx} {Λ : List (Res D)}
         have hr' : ∀ (σ : World D) (ρ : Env D _), _ := fun σ ρ => ihr σ ρ
         have he' : ∀ (σ : World D) (ρ : Env D _), _ := fun σ ρ => ihe σ ρ
         simp only [execBlock]
-        cases hein : einpassen (D.rtyp r) (O.regLies r σ) with
+        cases hein : einpassen O.zeiger (D.rtyp r) (O.regLies r σ) with
         | none => simp only [hein]
         | some v =>
             simp only [hein]
@@ -1367,7 +1367,7 @@ theorem armsOhneRuf_Runabhaengig {l : Bool} {Γ : Ctx} {Λ Λ' : List (Res D)}
     (fun r hk rest hr ihr σ ρ => by
         have hr' : ∀ (σ : World D) (ρ : Env D _), _ := fun σ ρ => ihr σ ρ
         simp only [execBlock]
-        cases hein : einpassen (D.rtyp r) (O.regLies r σ) with
+        cases hein : einpassen O.zeiger (D.rtyp r) (O.regLies r σ) with
         | none => simp only [hein]
         | some v =>
             simp only [hein]
@@ -1379,7 +1379,7 @@ theorem armsOhneRuf_Runabhaengig {l : Bool} {Γ : Ctx} {Λ Λ' : List (Res D)}
         have hr' : ∀ (σ : World D) (ρ : Env D _), _ := fun σ ρ => ihr σ ρ
         have he' : ∀ (σ : World D) (ρ : Env D _), _ := fun σ ρ => ihe σ ρ
         simp only [execBlock]
-        cases hein : einpassen (D.rtyp r) (O.regLies r σ) with
+        cases hein : einpassen O.zeiger (D.rtyp r) (O.regLies r σ) with
         | none => simp only [hein]
         | some v =>
             simp only [hein]
