grammatik/Grammatik/ZielOrtAxZeuge.lean
@@ -91,7 +91,7 @@ theorem axO_gut : GutO axO := by
     new value of the slot. -/
 theorem axO_vertrag : AxVertragO axQ axO := by
   intro a σ ρ v hv
-  have hv' : einpassen (.int 0 3) (axNeu σ).n = some v := hv
+  have hv' : einpassen axO.zeiger (.int 0 3) (axNeu σ).n = some v := hv
   simp only [einpassen, dif_pos (show 0 ≤ (axNeu σ).n ∧ (axNeu σ).n ≤ 3 from
     ⟨(axNeu σ).lo_le, (axNeu σ).le_hi⟩)] at hv'
   cases hv'
@@ -204,7 +204,7 @@ theorem axLauf : ∃ M : RufMaschineG axD,
     (fun _ _ => rfl) (fun e => nomatch e) (fun _ _ => axDarf) (fun e => nomatch e)
     (.cons (.ret (.wert (.var .hier)) (List.Perm.refl _)) .nil) (.dann .nil (.ende axRetNull)) .nil
     rfl _ axEins (by
-      show (_, einpassen (.int 0 3) (axNeu ((M3.weltVon 0).lese axL [])).n) = _
+      show (_, einpassen axO.zeiger (.int 0 3) (axNeu ((M3.weltVon 0).lese axL [])).n) = _
       have hn : (axNeu ((M3.weltVon 0).lese axL [])).n = 1 := by
         show min ((M3.speicher.slots () 0 ()).n + 1) 3 = 1
         rw [hsp3]
